start making progress on the linearizability example

theories/heap_lang/lifting.v
@@ -1,6 +1,6 @@
 From stdpp Require Import fin_maps.
 From iris.proofmode Require Import tactics.
-From iris.algebra Require Import auth excl agree gmap list.
+From iris.algebra Require Import auth excl excl_auth agree gmap list.
 From iris.algebra.lib Require Import frac_auth.
 From iris.base_logic Require Export gen_heap.
 From iris.base_logic.lib Require Export proph_map invariants.
@@ -39,17 +39,17 @@ Definition traceO := leibnizO (list val).
 Class traceG Σ := TraceG {
   trace_hist_inG :> inG Σ (authR (gmapUR nat (agreeR eventO)));
   trace_hist_name : gname;
-  trace_inG :> inG Σ (frac_authR (agreeR traceO));
+  trace_inG :> inG Σ (excl_authR traceO);
   trace_name : gname;
 }.
 
 Definition traceΣ : gFunctors :=
   #[GFunctor (authR (gmapUR nat (agreeR eventO)));
-    GFunctor (frac_authR (agreeR traceO))].
+    GFunctor (excl_authR traceO)].
 
 Class trace_preG Σ := TracePreG {
   trace_hist_preG_inG :> inG Σ (authR (gmapUR nat (agreeR eventO)));
-  trace_preG_inG :> inG Σ (frac_authR (agreeR traceO));
+  trace_preG_inG :> inG Σ (excl_authR traceO);
 }.
 
 Instance subG_tracePreG : subG traceΣ Σ → trace_preG Σ.
@@ -63,16 +63,14 @@ Class heapG Σ := HeapG {
 }.
 
 Definition trace_auth `{hT: traceG Σ} (t: list val) :=
-  (own trace_name (●F (to_agree (t: traceO))))%I.
+  (own trace_name (●E (t: traceO)))%I.
 Definition hist `{hT: traceG Σ} (t: list val) :=
   own trace_hist_name (◯ (gmap_of_trace 0 t)).
-Definition trace_half_frag `{hT:traceG} (t: list val) :=
-  own trace_name (◯F{1/2} (to_agree (t: traceO))).
 Definition trace_is `{hT: traceG Σ} (t: list val) :=
-  (trace_half_frag t ∗ own trace_hist_name (● gmap_of_trace 0 t) ∗ hist t)%I.
+  (own trace_name (◯E (t: traceO)) ∗ own trace_hist_name (● gmap_of_trace 0 t) ∗ hist t)%I.
 
-Definition trace_inv `{hT:traceG Σ, hI:invG Σ} (ι: namespace) (I: list val → Prop) :=
-  inv ι (∃ t, trace_half_frag t ∗ ⌜I t⌝).
+(* Definition trace_inv `{hT:traceG Σ, hI:invG Σ} (ι: namespace) (I: list val → Prop) t := *)
+(*   inv ι (trace_is t ∗ ⌜I t⌝). *)
 
 Instance hist_persistent `{traceG Σ} (t: list val): Persistent (hist t) := _.
 
@@ -82,51 +80,28 @@ Proof.
   rewrite /trace_is /hist. iIntros "(? & ? & #H)". iFrame "H ∗".
 Qed.
 
-Lemma trace_auth_half_frag_agree `{traceG Σ} t t':
-  trace_auth t -∗ trace_half_frag t' -∗ ⌜t = t'⌝.
-Proof.
-  rewrite /trace_auth /trace_is.
-  iIntros "H1 H2".
-  iDestruct (own_valid_2 with "H1 H2") as "H".
-  iDestruct "H" as %Hi%frac_auth_included.
-  rewrite -> Some_included_total in Hi.
-  apply to_agree_included, leibniz_equiv in Hi. eauto.
-Qed.
-
 Lemma trace_agree `{traceG Σ} t t':
   trace_auth t -∗ trace_is t' -∗ ⌜t = t'⌝.
 Proof.
-  iIntros "H1 (H2 & _ & _)". iApply (trace_auth_half_frag_agree with "H1 H2").
-Qed.
-
-Lemma trace_half_frag_agree `{traceG Σ} t t':
-  trace_half_frag t -∗ trace_is t' -∗ ⌜t = t'⌝.
-Proof.
-  rewrite /trace_is /trace_half_frag.
-  iIntros "H1 (H2 & _ & _)".
-  iDestruct (own_valid_2 with "H1 H2") as "H".
-  rewrite -frac_auth_frag_op Qp_half_half.
-  iDestruct "H" as %Hv. rewrite frac_auth_frag_valid in Hv |- * => Hv.
-  destruct Hv as [_ Hv]. apply agree_op_inv', leibniz_equiv in Hv. eauto.
+  rewrite /trace_auth /trace_is.
+  iIntros "H1 (H2 & _)".
+  iDestruct (own_valid_2 with "H1 H2") as %HH. by apply excl_auth_agree in HH.
 Qed.
 
 Lemma trace_add_event `{traceG Σ} t (v: val) :
-  trace_auth t -∗ trace_is t -∗ trace_half_frag t ==∗
-  trace_auth (t ++ [v]) ∗ trace_is (t ++ [v]) ∗ trace_half_frag (t ++ [v]).
+  trace_auth t -∗ trace_is t ==∗
+  trace_auth (t ++ [v]) ∗ trace_is (t ++ [v]).
 Proof.
   rewrite /trace_auth /trace_is /hist.
-  iIntros "H1 (H2 & H2ha & H2h) H3".
-  iDestruct (own_op with "[$H2 $H3]") as "H2".
-  rewrite -frac_auth_frag_op Qp_half_half agree_idemp.
-  iMod (own_update_2 _ _ _ (●F (to_agree (t++[v]:traceO)) ⋅ ◯F (to_agree (t++[v]:traceO))) with "H1 H2") as "[? ?]".
-  by apply frac_auth_update_1.
+  iIntros "H1 (H2 & H2ha & H2h)".
+  iMod (own_update_2 _ _ _ (●E (t++[v]:traceO) ⋅ ◯E (t++[v]:traceO)) with "H1 H2") as "[? ?]".
+  by apply excl_auth_update.
   rewrite gmap_of_trace_snoc Nat.add_0_l.
   iMod (own_update_2 with "H2ha H2h") as "[? ?]".
   apply auth_update.
   eapply (alloc_local_update _ _ (length t : nat) (to_agree (v:eventO))); [|done].
   { eapply not_elem_of_dom. intros ?%gmap_of_trace_dom. lia. }
   iModIntro. iFrame.
-  rewrite /trace_half_frag -own_op -frac_auth_frag_op Qp_half_half agree_idemp //.
   Unshelve. all: typeclasses eauto.
 Qed.
 
@@ -172,14 +147,13 @@ Proof.
   iPureIntro. eapply gmap_of_trace_hist_valid_prefix; eauto.
 Qed.
 
-Lemma trace_is_inv `{traceG Σ, invG Σ} t N I :
-  trace_is t -∗ trace_inv N I ={⊤}=∗ trace_is t ∗ ⌜ I t ⌝.
-Proof.
-  iIntros "Ht Hi". unfold trace_inv.
-  iInv N as ">H" "Hclose". iDestruct "H" as (t') "(Ht' & %)".
-  iDestruct (trace_half_frag_agree with "[$] [$]") as %->.
-  iMod ("Hclose" with "[Ht']"). eauto. iIntros "!>". eauto.
-Qed.
+(* Lemma trace_inv_pure `{traceG Σ, invG Σ} t N I : *)
+(*   trace_inv N I t ={⊤}=∗ ⌜ I t ⌝. *)
+(* Proof. *)
+(*   iIntros "Hi". unfold trace_inv. *)
+(*   iInv N as ">H" "Hclose". iDestruct "H" as "(Ht' & %)". *)
+(*   iMod ("Hclose" with "[Ht']"). eauto. iIntros "!>". eauto. *)
+(* Qed. *)
 
 Lemma gmap_of_trace_valid {A} (l: list A) (n: nat):
   ✓ gmap_of_trace n l.
@@ -190,17 +164,15 @@ Proof.
 Qed.
 
 Lemma trace_auth_init `{hT: trace_preG Σ} (t: list val) :
-  ⊢ |==> ∃ H: traceG Σ, trace_auth t ∗ trace_is t ∗ trace_half_frag t.
+  ⊢ |==> ∃ H: traceG Σ, trace_auth t ∗ trace_is t.
 Proof.
-  iMod (own_alloc (●F (to_agree (t: traceO)) ⋅ ◯F (to_agree (t: traceO)))) as (γ) "Hγ".
-  by apply frac_auth_valid.
+  iMod (own_alloc (●E (t: traceO) ⋅ ◯E (t: traceO))) as (γ) "Hγ".
+  by apply excl_auth_valid.
   rewrite own_op. iDestruct "Hγ" as "[? Hγf]".
   iMod (own_alloc (● gmap_of_trace 0 t ⋅ ◯ gmap_of_trace 0 t)) as (γh) "Hγh".
   apply auth_both_valid. split; [ done | by apply gmap_of_trace_valid].
   rewrite own_op. iDestruct "Hγh" as "[? ?]".
-  iModIntro. iExists (TraceG _ _ γh _ γ).
-  rewrite /trace_auth /trace_is /trace_half_frag /hist. iFrame.
-  rewrite -own_op -frac_auth_frag_op Qp_half_half agree_idemp //.
+  iModIntro. iExists (TraceG _ _ γh _ γ). iFrame.
 Qed.
 
 Instance heapG_irisG `{!heapG Σ} : irisG heap_lang Σ := {
@@ -413,26 +385,40 @@ Implicit Types σ : state.
 Implicit Types v : val.
 Implicit Types l : loc.
 
-Lemma wp_emit s E tr v ι (I: list val → Prop) :
-  ↑ι ⊆ E →
-  I (tr ++ [v]) →
-  {{{ trace_is tr ∗ trace_inv ι I }}}
+Lemma wp_emit s E tr v :
+  {{{ trace_is tr }}}
     Emit v @ s; E
   {{{ RET (LitV LitUnit); trace_is (tr ++ [v]) }}}.
 Proof.
-  iIntros (Hι HI φ) "[Ht Hi] Hφ".
-  iInv "Hi" as ">Hi" "Hclose".
-  iDestruct "Hi" as (tr') "[Htr' _]".
-  iDestruct (trace_half_frag_agree with "Htr' Ht") as %->.
+  iIntros (φ) "Ht Hφ".
   iApply wp_lift_atomic_head_step; [done|].
   iIntros (σ1 κ κs n) "(? & Hta & ?) !>"; iSplit; first by eauto.
   iNext. iIntros (v2 σ2 efs Hstep); inv_head_step.
   iDestruct (trace_agree with "Hta Ht") as %<-.
-  iMod (trace_add_event with "Hta Ht Htr'") as "(Hta&Ht&Htr')".
+  iMod (trace_add_event with "Hta Ht") as "(Hta&Htr')".
   iModIntro. iFrame. iSplitL; last done.
-  iMod ("Hclose" with "[Htr']"). { iNext. eauto. }
-  iModIntro. by iApply "Hφ".
+  by iApply "Hφ".
 Qed.
+
+(* Lemma wp_emit_inv s E tr v N (I: list val → Prop) : *)
+(*   ↑N ⊆ E → *)
+(*   I (tr ++ [v]) → *)
+(*   {{{ trace_inv N I tr }}} *)
+(*     Emit v @ s; E *)
+(*   {{{ RET (LitV LitUnit); trace_inv N I (tr ++ [v]) }}}. *)
+(* Proof. *)
+(*   iIntros (? HI φ) "Ht Hφ". *)
+(*   iInv N as ">(H & %)" "Hclose". *)
+(*   iApply (wp_emit with "H"). iIntros "!> Ht". *)
+
+(*   iApply wp_lift_atomic_head_step; [done|]. *)
+(*   iIntros (σ1 κ κs n) "(? & Hta & ?) !>"; iSplit; first by eauto. *)
+(*   iNext. iIntros (v2 σ2 efs Hstep); inv_head_step. *)
+(*   iDestruct (trace_agree with "Hta Ht") as %<-. *)
+(*   iMod (trace_add_event with "Hta Ht") as "(Hta&Htr')". *)
+(*   iModIntro. iFrame. iSplitL; last done. *)
+(*   by iApply "Hφ". *)
+(* Qed. *)
 
 Lemma pick_fresh_tag (tr: list val) :
   ∃ (tag: string), fresh_tag tag tr.
@@ -452,26 +438,20 @@ Proof.
   eexists. split; eauto. reflexivity.
 Qed.
 
-Lemma wp_fresh s E tr v ι (I: list val → Prop) :
-  ↑ι ⊆ E →
-  (∀ tag, fresh_tag tag tr → I (tr ++ [(#tag, v)%V])) →
-  {{{ trace_is tr ∗ trace_inv ι I }}}
+Lemma wp_fresh s E tr v :
+  {{{ trace_is tr }}}
     Fresh v @ s; E
-  {{{ (tag:string), RET (LitV tag); trace_is (tr ++ [(#tag, v)%V]) }}}.
+  {{{ (tag:string), RET (LitV tag); trace_is (tr ++ [(#tag, v)%V]) ∗ ⌜fresh_tag tag tr⌝ }}}.
 Proof.
-  iIntros (Hι HI φ) "[Ht Hi] Hφ".
-  iInv "Hi" as ">Hi" "Hclose".
-  iDestruct "Hi" as (tr') "[Htr' _]".
-  iDestruct (trace_half_frag_agree with "Htr' Ht") as %->.
+  iIntros (φ) "Ht Hφ".
   iApply wp_lift_atomic_head_step; [done|].
   iIntros (σ1 κ κs n) "(? & Hta & ?) !>".
   destruct (pick_fresh_tag σ1.(trace)) as [tag Htag]. iSplit; [ by eauto |].
   iNext. iIntros (v2 σ2 efs Hstep); inv_head_step.
   iDestruct (trace_agree with "Hta Ht") as %<-.
-  iMod (trace_add_event with "Hta Ht Htr'") as "(Hta & Ht & Htr')".
+  iMod (trace_add_event with "Hta Ht") as "(Hta & Htr')".
   iModIntro. iFrame. iSplitL; last done.
-  iMod ("Hclose" with "[Htr']"). { iNext. eauto. }
-  iModIntro. by iApply "Hφ".
+  iApply "Hφ". eauto.
 Qed.
 
 (** Fork: Not using Texan triples to avoid some unnecessary [True] *)
