theories/heap_lang/adequacy.v
@@ -30,62 +30,62 @@ Proof.
   iFrame. iApply (Hwp (HeapG _ _ _ _ _)).
 Qed.
 
-Definition heap_invariance Σ `{!heapPreG Σ} (N: namespace) (I: list val → Prop) s e σ :
-  I (trace σ) →
-  (∀ `{!heapG Σ}, ⊢ trace_inv N I -∗ trace_is (trace σ) -∗ WP e @ s; ⊤ {{ _, True }}) →
-  ∀ σ' t,
-    rtc erased_step ([e], σ) (t, σ') →
-    I (trace σ').
-Proof.
-  intros HI Hwp σ' t.
-  eapply (wp_invariance Σ _ s _ _ _ _ (I (trace σ'))). iIntros (Hinv κs) "".
-  iMod (gen_heap_init σ.(heap)) as (?) "Hh".
-  iMod (proph_map_init κs σ.(used_proph_id)) as (?) "Hp".
-  iMod (trace_auth_init σ.(trace)) as (?) "(Hta & Ht & Hth)".
-  iDestruct (inv_alloc N _ (∃ t, trace_half_frag t ∗ ⌜I t⌝) with "[Hth]") as ">#HI".
-  { iNext. eauto. }
-  iModIntro. iExists
-    (λ σ κs _, (gen_heap_ctx σ.(heap) ∗ trace_auth σ.(trace) ∗ proph_map_ctx κs σ.(used_proph_id))%I),
-    (λ _, True%I).
-  iFrame. iSplitL.
-  { iDestruct (Hwp (HeapG _ _ _ _ _)) as "Hwp". iApply ("Hwp" with "HI Ht"). }
-  iIntros "(_ & Hta & _)". iExists _.
-  iInv "HI" as ">Ht'" "_". iDestruct "Ht'" as (t') "(Ht' & %)".
-  iDestruct (trace_auth_half_frag_agree with "Hta Ht'") as %->. iModIntro. eauto.
-Qed.
+(* Definition heap_invariance Σ `{!heapPreG Σ} (N: namespace) (I: list val → Prop) s e σ : *)
+(*   I (trace σ) → *)
+(*   (∀ `{!heapG Σ}, ⊢ trace_inv N I -∗ trace_is (trace σ) -∗ WP e @ s; ⊤ {{ _, True }}) → *)
+(*   ∀ σ' t, *)
+(*     rtc erased_step ([e], σ) (t, σ') → *)
+(*     I (trace σ'). *)
+(* Proof. *)
+(*   intros HI Hwp σ' t. *)
+(*   eapply (wp_invariance Σ _ s _ _ _ _ (I (trace σ'))). iIntros (Hinv κs) "". *)
+(*   iMod (gen_heap_init σ.(heap)) as (?) "Hh". *)
+(*   iMod (proph_map_init κs σ.(used_proph_id)) as (?) "Hp". *)
+(*   iMod (trace_auth_init σ.(trace)) as (?) "(Hta & Ht & Hth)". *)
+(*   iDestruct (inv_alloc N _ (∃ t, trace_half_frag t ∗ ⌜I t⌝) with "[Hth]") as ">#HI". *)
+(*   { iNext. eauto. } *)
+(*   iModIntro. iExists *)
+(*     (λ σ κs _, (gen_heap_ctx σ.(heap) ∗ trace_auth σ.(trace) ∗ proph_map_ctx κs σ.(used_proph_id))%I), *)
+(*     (λ _, True%I). *)
+(*   iFrame. iSplitL. *)
+(*   { iDestruct (Hwp (HeapG _ _ _ _ _)) as "Hwp". iApply ("Hwp" with "HI Ht"). } *)
+(*   iIntros "(_ & Hta & _)". iExists _. *)
+(*   iInv "HI" as ">Ht'" "_". iDestruct "Ht'" as (t') "(Ht' & %)". *)
+(*   iDestruct (trace_auth_half_frag_agree with "Hta Ht'") as %->. iModIntro. eauto. *)
+(* Qed. *)
 
-Require Import iris.program_logic.hoare.
+(* Require Import iris.program_logic.hoare. *)
 
-Lemma module_invariance {Σ} `{heapPreG Σ} (N: namespace)
-  (Φ: ∀ `{heapG Σ}, iProp Σ → val → iProp Σ)  (* Module specification *)
-  (P0: iProp Σ) (* Initial resources required by the module *)
-  (e: val → expr) (* Context program, parameterized by the module *)
-  (e_init: expr) (* Initialization code, used to allocate resources for P0 *)
-  (imimpl: val) (* Implementation of the module (instrumented) *)
-  (good_trace: list val → Prop) (* Trace property *)
-  (σ: state) (* Initial state *)
-:
-  (* The initial trace must satisfy the property *)
-  good_trace (trace σ) →
-  (* The context must be safe, given a module satisfying the specification Φ *)
-  (⊢ ∀ `{heapG Σ} P m, Φ P m -∗ {{{ P }}} e m {{{ v, RET v; True }}}) →
-  (* The initialization code must provide P0 *)
-  (⊢ ∀ `{heapG Σ}, {{ True }} e_init {{ _, P0 }}) →
-  (* The implementation provided for the module (iops) must satisfy the specification Φ.
-     On top of P0 it is given SL resources for the trace. *)
-  (⊢ ∀ `{heapG Σ}, Φ (P0 ∗ trace_is (trace σ) ∗ trace_inv N good_trace)%I imimpl) →
-  (* Then the trace remains good at every step *)
-  ∀ σ' e',
-    rtc erased_step ([(e_init;; e imimpl)%E], σ) (e', σ') →
-    good_trace (trace σ').
-Proof.
-  intros Htrσ Hctx Hinit Himpl σ' e' Hsteps.
-  eapply heap_invariance. done. by apply Htrσ. 2: eapply Hsteps.
-  iIntros (?) "HI Htr". wp_bind e_init.
-  iApply wp_wand. by iApply Hinit.
-  iIntros (v) "H0". wp_pures.
-  iApply (Hctx with "[] [H0 Htr HI]").
-  - iApply Himpl.
-  - iFrame.
-  - eauto.
-Qed.
+(* Lemma module_invariance {Σ} `{heapPreG Σ} (N: namespace) *)
+(*   (Φ: ∀ `{heapG Σ}, iProp Σ → val → iProp Σ)  (* Module specification *) *)
+(*   (P0: iProp Σ) (* Initial resources required by the module *) *)
+(*   (e: val → expr) (* Context program, parameterized by the module *) *)
+(*   (e_init: expr) (* Initialization code, used to allocate resources for P0 *) *)
+(*   (imimpl: val) (* Implementation of the module (instrumented) *) *)
+(*   (good_trace: list val → Prop) (* Trace property *) *)
+(*   (σ: state) (* Initial state *) *)
+(* : *)
+(*   (* The initial trace must satisfy the property *) *)
+(*   good_trace (trace σ) → *)
+(*   (* The context must be safe, given a module satisfying the specification Φ *) *)
+(*   (⊢ ∀ `{heapG Σ} P m, Φ P m -∗ {{{ P }}} e m {{{ v, RET v; True }}}) → *)
+(*   (* The initialization code must provide P0 *) *)
+(*   (⊢ ∀ `{heapG Σ}, {{ True }} e_init {{ _, P0 }}) → *)
+(*   (* The implementation provided for the module (iops) must satisfy the specification Φ. *)
+(*      On top of P0 it is given SL resources for the trace. *) *)
+(*   (⊢ ∀ `{heapG Σ}, Φ (P0 ∗ trace_is (trace σ) ∗ trace_inv N good_trace)%I imimpl) → *)
+(*   (* Then the trace remains good at every step *) *)
+(*   ∀ σ' e', *)
+(*     rtc erased_step ([(e_init;; e imimpl)%E], σ) (e', σ') → *)
+(*     good_trace (trace σ'). *)
+(* Proof. *)
+(*   intros Htrσ Hctx Hinit Himpl σ' e' Hsteps. *)
+(*   eapply heap_invariance. done. by apply Htrσ. 2: eapply Hsteps. *)
+(*   iIntros (?) "HI Htr". wp_bind e_init. *)
+(*   iApply wp_wand. by iApply Hinit. *)
+(*   iIntros (v) "H0". wp_pures. *)
+(*   iApply (Hctx with "[] [H0 Htr HI]"). *)
+(*   - iApply Himpl. *)
+(*   - iFrame. *)
+(*   - eauto. *)
+(* Qed. *)
