theories/linearizability.v
@@ -1,0 +1,256 @@
+From iris.proofmode Require Import tactics.
+From iris.algebra Require Import auth excl excl_auth.
+From iris.base_logic.lib Require Import invariants.
+From iris.program_logic Require Import atomic.
+From intensional.heap_lang Require Import lifting proofmode notation.
+From intensional.heap_lang Require Import adequacy.
+From intensional Require Import stdpp_extra tactics.
+Set Default Proof Using "Type".
+Implicit Types t : list val.
+
+Class model := {
+  S :> Type;
+  s_init : S;
+  f : S → val → S;
+  r : S → val → val;
+}.
+
+Section Specs.
+Context `{!heapG Σ}.
+Context `{model}.
+Context (E: coPset).
+Context (Pinit: iProp Σ)
+        (is_P: gname → val → iProp Σ)
+        (P_content: gname → S → iProp Σ).
+
+Definition init_spec (init: val) : iProp Σ :=
+  {{{ Pinit }}} init {{{ γ r, RET r; is_P γ r ∗ P_content γ s_init }}}.
+
+Definition op_spec (op: val) : iProp Σ :=
+  ∀ γ (x y: val),
+    is_P γ x -∗
+    <<< ∀ s, P_content γ s >>>
+      op x y @ ⊤∖E
+    <<< P_content γ (f s y), RET (r s y) >>>.
+
+Definition lib_spec (lib: val) : iProp Σ :=
+  ⌜∀ γ x, Persistent (is_P γ x)⌝ ∗
+  ⌜∀ γ s, Timeless (P_content γ s)⌝ ∗
+  ⌜∀ γ s1 s2, P_content γ s1 -∗ P_content γ s2 -∗ False⌝ ∗
+  match lib with
+  | (init, op)%V => init_spec init ∗ op_spec op
+  | _ => False
+  end.
+
+End Specs.
+
+Section Trace.
+
+(* Inductive concurrent_trace : list val → Prop := *)
+(*   | concurrent_trace_nil : *)
+(*       concurrent_trace [] *)
+(*   | concurrent_trace_call (tag: string) (v: val) t : *)
+(*       concurrent_trace t → *)
+(*       concurrent_trace (t ++ [(#tag, (#"call", v))%V]) *)
+(*   | concurrent_trace_ret (tag: string) (v v': val) t : *)
+(*       concurrent_trace t → *)
+(*       concurrent_trace (t ++ [(#tag, (#"ret", (v, v')))%V]). *)
+
+Inductive linearization_trace : list val → Prop :=
+  | linearization_trace_nil :
+      linearization_trace []
+  | linearization_trace_call (tag: string) (v: val) t :
+      linearization_trace t →
+      linearization_trace (t ++ [(#tag, (#"call", v))%V])
+  | linearization_trace_lin (tag: string) (v v': val) t :
+      linearization_trace t →
+      linearization_trace (t ++ [(#tag, (#"lin", (v, v')))%V])
+  | linearization_trace_ret (tag: string) (v v': val) t :
+      linearization_trace t →
+      linearization_trace (t ++ [(#tag, (#"ret", (v, v')))%V]).
+
+Inductive linearized_trace_for (tag: string) : list val → Prop :=
+  | linearized_trace_for_nil :
+      linearized_trace_for tag []
+  | linearized_trace_for_call t (v v': val) :
+      linearized_trace_for tag t →
+      linearized_trace_for tag (t ++ [(#tag, (#"call", v)); (#tag, (#"lin", (v, v'))); (#tag, (#"ret", (v, v')))]%V).
+
+Inductive linearized_sound `{model} : list val → S → S → Prop :=
+  (* administrative steps. calls and rets are ignored. *)
+  | linearized_sound_nil s :
+      linearized_sound [] s s
+  | linearized_sound_call_ret s0 s (tag op: string) arg t :
+      linearized_sound t s0 s →
+      op = "call" ∨ op = "ret" →
+      linearized_sound (t ++ [(#tag, (#op, arg))%V]) s0 s
+  (* lin events must be sound wrt the model *)
+  | linearized_sound_lin s0 s (tag:string) v v' t :
+      linearized_sound t s0 s →
+      v' = r s v →
+      linearized_sound (t ++ [(#tag, (#"lin", (v, v')))%V]) s0 (f s v).
+
+Inductive matching_call_ret : list val → list val → Prop :=
+  | matching_call_ret_nil t' :
+      matching_call_ret [] t'
+  | matching_call_ret_lin t t' (tag: string) v v':
+      matching_call_ret t t' →
+      matching_call_ret t (t' ++ [(#tag, (#"lin", (v, v')))%V])
+  | matching_call_ret_call t t' (tag: string) v :
+      matching_call_ret t t' →
+      matching_call_ret (t ++ [(#tag, (#"call", v))%V]) (t' ++ [(#tag, (#"call", v))%V])
+  | matching_call_ret_ret t t' (tag: string) v v' :
+      matching_call_ret t t' →
+      matching_call_ret (t ++ [(#tag, (#"ret", (v, v')))%V]) (t' ++ [(#tag, (#"ret", (v, v')))%V])
+.
+
+Definition check_tag (tag: string) (v: val) :=
+  match v with
+  | (# (LitTag tag'), _)%V => String.eqb tag tag'
+  | _ => false
+  end.
+
+Definition linearizable `{model} t :=
+  ∃ t', linearization_trace t'
+        ∧ (∀ tag, linearized_trace_for tag (filter (check_tag tag) t'))
+        ∧ matching_call_ret t t'
+        ∧ ∃ s', linearized_sound t' s_init s'.
+
+End Trace.
+
+Module Wrap.
+Section S.
+Context {Σ: gFunctors}.
+Context `{heapG Σ}.
+Context (N N': namespace) (HNN': N ## N').
+Context `{model}.
+Context `{inG Σ (excl_authR (leibnizO S))}
+        `{inG Σ (excl_authR (leibnizO (gname * gname)))}.
+
+Local Notation SO := (leibnizO S).
+
+Context (Pinit_impl: iProp Σ)
+        (is_P_impl: gname → val → iProp Σ)
+        (P_content_impl: gname → S → iProp Σ).
+Context (HPP: ∀ γ x, Persistent (is_P_impl γ x)).
+Context (HPT: ∀ γ s, Timeless (P_content_impl γ s)).
+
+Context (init_impl op_impl : val).
+
+Definition init : val :=
+  init_impl.
+
+Definition op : val :=
+  λ: "x" "y",
+    let: "t" := Fresh (#"call", "y") in
+    let: "r" := op_impl "x" "y" in
+    Emit ("t", (#"ret", ("y", "r"))) ;;
+    "r".
+
+Definition Pinit : iProp Σ :=
+  Pinit_impl ∗ trace_is [].
+
+Definition is_call_return (v: val) :=
+  match v with
+  | (#_, (#"call", _))%V | (#_, (#"ret", _))%V => true
+  | _ => false
+  end.
+
+Definition trace_inv (γ: gname) (s: S) : iProp Σ :=
+  ∃ (β: list val),
+    ⌜linearization_trace β⌝ ∗
+    ⌜linearized_sound β s_init s⌝ ∗
+    trace_is (filter is_call_return β) ∗
+    own γ (●E (s:SO)).
+
+Definition is_P γ x : iProp Σ :=
+    is_P_impl γ(*XXX*) x ∗
+    inv N' (∃ s, trace_inv γ s).
+
+Definition P_content γ s : iProp Σ :=
+  P_content_impl γ(*XXX*) s ∗
+  own γ (◯E (s:SO)).
+
+Lemma excl_agree_eq A `{inG Σ (excl_authR (leibnizO A))} γ (x y: A):
+  own γ (◯E (x:leibnizO A)) -∗ own γ (●E (y:leibnizO A)) -∗ ⌜x = y⌝.
+Proof.
+  iIntros "H1 H2". iDestruct (own_op with "[$H1 $H2]") as "H".
+  iDestruct (own_valid with "H") as %HH%excl_auth_agree. done.
+Qed.
+
+Lemma excl_auth_upd A `{inG Σ (excl_authR (leibnizO A))} γ (x y z: A):
+  own γ (◯E (x:leibnizO A)) -∗ own γ (●E (y:leibnizO A)) ==∗
+  own γ (◯E (z:leibnizO A)) ∗ own γ (●E (z:leibnizO A)).
+Proof.
+  iIntros "H1 H2". SearchAbout own "_2".
+  iDestruct (own_update_2 with "H1 H2") as ">[? ?]".
+  apply excl_auth_update. iModIntro. iFrame.
+Qed.
+
+(* Lemma init_correct : *)
+(*   init_spec Pinit_impl is_P_impl P_content_impl init_impl -∗ *)
+(*   init_spec Pinit is_P P_content init. *)
+(* Proof. *)
+(*   iIntros "#spec" (φ) "!> (Hi & Ht) Hφ". unfold init. *)
+(*   iApply ("spec" with "Hi"). iIntros "!>" (γ x) "(Hi & Hc)". *)
+(*   iApply "Hφ". iFrame. *)
+
+
+
+Lemma op_correct :
+  op_spec (↑N) is_P_impl P_content_impl op_impl -∗
+  op_spec (↑N ∪ ↑N') is_P P_content op.
+Proof using HPT HPP HNN'.
+  iIntros "spec" (γ x y) "(#H1 & #H2)".
+  iIntros (φ) "HAU".
+  unfold op. wp_pures. wp_bind (Fresh _). unfold op_spec.
+  iInv N' as ">Ht" "Hclose". iDestruct "Ht" as (s β) "(% & % & Ht & Hγ)".
+  iApply (wp_fresh with "Ht"). iNext. iIntros (tag) "(Ht & %)".
+  iMod ("Hclose" with "[Ht Hγ]") as "_".
+  { iNext. iExists s. unfold trace_inv at 2.
+    iExists (β ++ [(#tag, (#"call", y))%V])(*XXX*).
+    iSplitR. iPureIntro; by constructor.
+    iSplitR. iPureIntro; by constructor; eauto.
+    iFrame. rewrite filter_app //=. }
+  iModIntro. wp_pures. clear dependent s β.
+
+  iSpecialize ("spec" $! _ _ y with "H1").
+  awp_apply "spec".
+
+  rewrite /atomic_acc /=.
+  iInv N' as ">HI" "Hclose". iDestruct "HI" as (s) "HI".
+  iMod "HAU" as (s') "(HH & Hnext)". by set_solver.
+  iDestruct "HH" as "(HHi & HHa)".
+  iModIntro. iExists _. iFrame "HHi".
+  iSplit.
+  { (* abort case *)
+    iIntros "HHi". iDestruct "Hnext" as "[Hnext _]".
+    iSpecialize ("Hnext" with "[$HHi $HHa]").
+    iMod "Hnext". iMod ("Hclose" with "[HI]") as "_"; eauto. }
+
+  (* continue case *)
+  iIntros "HHi". iDestruct "Hnext" as "[_ Hnext]".
+  iDestruct "HI" as (β) "(% & % & Ht & HHf)".
+  iDestruct (excl_agree_eq with "HHa HHf") as %->.
+  iDestruct (excl_auth_upd _ _ _ _ (f s y) with "HHa HHf") as ">[HHa HHf]".
+  iSpecialize ("Hnext" with "[$HHi $HHa]"). iMod "Hnext".
+  iMod ("Hclose" with "[Ht HHf]") as "_".
+  { iNext. iExists _. unfold trace_inv at 2.
+    iExists (β ++ [(#tag, (#"lin", (y, r s y)))%V]). iFrame.
+    rewrite filter_app app_nil_r. iFrame. iPureIntro. split.
+    { by constructor. }
+    { by eapply linearized_sound_lin. } }
+
+  iModIntro. wp_pures. wp_bind (Emit _).
+  iInv N' as ">HI" "Hclose". iDestruct "HI" as (s' β') "(% & % & Ht & HHf)".
+  iApply (wp_emit with "Ht"). iIntros "!> Ht".
+  iMod ("Hclose" with "[HHf Ht]").
+  { iNext. iExists _. unfold trace_inv at 2.
+    iExists (β' ++ [(#tag, (#"ret", (y, r s y)))%V]). iFrame.
+    rewrite filter_app. iFrame. iPureIntro. split.
+    { by constructor. }
+    { by constructor; eauto. } }
+
+  iModIntro. wp_pures. eauto.
+Qed.
+
